lib/Benchmarks/EthernetProof.v
@@ -7,26 +7,23 @@ Notation conf := (P4automaton.configuration (P4A.interp A)).
 Notation start_left := Reference.SPref.
 Notation start_right := Combined.Parse.
 
-Definition r_states :=
-  Eval vm_compute in (Reachability.reachable_states
-                        A
-                        200
-                        start_left
-                        start_right).
+Definition r_states : {r : Reachability.state_pairs A & Reachability.reachable_states_wit start_left start_right r}.
+  econstructor.
+  unfold Reachability.reachable_states_wit.
+  solve_fp_wit.
+Defined.
+
+Lemma init_states_wf:
+  Reachability.valid_state_pair (Reachability.build_state_pair A start_left start_right).
+Proof.
+  vm_compute; Lia.lia.
+Qed.
 
 Definition top : Relations.rel conf := fun _ _ => True.
 Definition top' : Relations.rel (state_template A) := fun _ _ => True.
 
 Declare ML Module "mirrorsolve".
-
-(*
-RegisterEnvCtors
-  (Reference.HPref, FirstOrderConfRelSimplified.Bits 64)
-  (Reference.HSrc, FirstOrderConfRelSimplified.Bits 48)
-  (Reference.HDest, FirstOrderConfRelSimplified.Bits 48)
-  (Reference.HProto, FirstOrderConfRelSimplified.Bits 16)
-  (Combined.HdrVar, FirstOrderConfRelSimplified.Bits 176).
-*)
+(* SetSMTSolver "cvc4". *)
 
 Lemma prebisim_incremental_sep:
   forall q1 q2,
@@ -44,21 +41,26 @@ Lemma prebisim_incremental_sep:
                       cr_rel := btrue;
                    |} q1 q2 ->
   pre_bisimulation A
-                   (wp r_states)
+                   (wp (projT1 r_states))
                    top
                    []
-                   (mk_init _ _ _ _ A 200 start_left start_right)
+                   (mk_init _ _ _ _ A start_left start_right)
                    q1 q2.
 Proof.
   idtac "running ethernet bisimulation".
-
   intros.
-  set (a := A).
-  set (rel0 := (mk_init _ _ _ _ _ _ _ _)).
-  vm_compute in rel0.
-  subst rel0.
 
-  time "build phase" repeat (time "single step" run_bisim top top' r_states).
+  pose proof (Reachability.reachable_states_wit_conv init_states_wf (projT2 r_states)) as Hr.
+
+  unfold mk_init.
+  rewrite Hr.
+  clear Hr.
+  
+  set (foo := (List.nodup (conf_rel_eq_dec (a:=A)) (mk_partition _ _ _ _ _ _))).
+  vm_compute in foo.
+  subst foo.
+
+  time "build phase" repeat (time "single step" run_bisim top top' (projT1 r_states)).
   time "close phase" close_bisim top'.
 
 Time Admitted.
