lib/Benchmarks/ServiceproviderSelfProof.v
@@ -12,69 +12,24 @@ Notation conf := (P4automaton.configuration (P4A.interp A)).
 Notation start_left := (Plain.ParseEth).
 Notation start_right := (Plain.ParseEth).
 
-Notation r_len := 9.
-(* Fixpoint reachable_states_len' (r: Reachability.state_pairs A) (acc: nat) (fuel: nat) :=
-  match fuel with
-  | 0 => None
-  | S x =>
-    let nxt := Reachability.reachable_step r in
-    let nxt_len := length nxt in
-    if Nat.eq_dec (length nxt) (length r) then Some acc
-    else
-      reachable_states_len' nxt (S acc) x
-  end.
+Definition r_states : {r : Reachability.state_pairs A & Reachability.reachable_states_wit start_left start_right r}.
+  econstructor.
+  unfold Reachability.reachable_states_wit.
+  solve_fp_wit.
+Defined.
 
-Definition reachable_states_len : nat.
-  refine (
-  let s := ({| st_state := inl (inl start_left); st_buf_len := 0 |},
-            {| st_state := inl (inr start_right); st_buf_len := 0 |}) in
-  let r := reachable_states_len' [s] 0 1000 in
-  _).
-  vm_compute in r.
-  match goal with
-  | _ := Some ?x |- _ => exact x
-  end.
-  Defined.
-Print reachable_states_len. *)
-
-Definition r_states : list (Reachability.state_pair A) :=
-  Eval vm_compute in (Reachability.reachable_states
-                        A
-                        r_len
-                        start_left
-                        start_right).
+Lemma init_states_wf:
+  Reachability.valid_state_pair (Reachability.build_state_pair A start_left start_right).
+Proof.
+  vm_compute; Lia.lia.
+Qed.
 
 Definition top : Relations.rel conf := fun _ _ => True.
 Definition top' : Relations.rel (state_template A) := fun _ _ => True.
 
 ClearEnvCtors.
 
-(*
-| HdrEth: header eth_size
-| HdrMPLS0: header mpls_size
-| HdrMPLS1: header mpls_size
-| HdrMPLS2: header mpls_size
-| HdrMPLS3: header mpls_size
-| HdrMPLS4: header mpls_size
-| HdrMPLS5: header mpls_size
-| HdrIPVer: header 4
-| HdrIPv4: header ipv4_size
-| HdrIPv6: header ipv6_size
- *)
-
-(*
-RegisterEnvCtors
-  (HdrEth, FirstOrderConfRelSimplified.Bits eth_size)
-  (HdrMPLS0, FirstOrderConfRelSimplified.Bits mpls_size)
-  (HdrMPLS1, FirstOrderConfRelSimplified.Bits mpls_size)
-  (HdrMPLS2, FirstOrderConfRelSimplified.Bits mpls_size)
-  (HdrMPLS3, FirstOrderConfRelSimplified.Bits mpls_size)
-  (HdrMPLS4, FirstOrderConfRelSimplified.Bits mpls_size)
-  (HdrMPLS5, FirstOrderConfRelSimplified.Bits mpls_size)
-  (HdrIPVer, FirstOrderConfRelSimplified.Bits 4)
-  (HdrIPv4, FirstOrderConfRelSimplified.Bits ipv4_size)
-  (HdrIPv6, FirstOrderConfRelSimplified.Bits ipv4_size).
-*)
+SetSMTSolver "cvc4".
 
 Lemma prebisim_babyip:
   forall q1 q2,
@@ -92,20 +47,26 @@ Lemma prebisim_babyip:
                       cr_rel := btrue;
                   |} q1 q2 ->
   pre_bisimulation A
-                  (wp r_states)
+                  (wp (projT1 r_states))
                   top
                   []
-                  (mk_init _ _ _ _ A r_len start_left start_right)
+                  (mk_init _ _ _ _ A start_left start_right)
                   q1 q2.
 Proof.
   idtac "running edge self-comparison bisimulation".
 
   intros.
-  set (rel0 := (mk_init _ _ _ _ _ _ _ _)).
+  pose proof (Reachability.reachable_states_wit_conv init_states_wf (projT2 r_states)) as Hr.
+
+  unfold mk_init.
+  rewrite Hr.
+  clear Hr.
+  
+  set (rel0 := (List.nodup _) (mk_partition _ _ _ _ _ _)).
   vm_compute in rel0.
   subst rel0.
 
-  time "build phase" repeat (time "single step" run_bisim top top' r_states).
+  time "build phase" repeat (time "single step" run_bisim top top' (projT1 r_states)).
 
   (* run_bisim top top' r_states. *)
   time "close phase" close_bisim top'.
